src/michocoq/main.v
@@ -1,8 +1,14 @@
 Require Import String ZArith.
 Require micheline_lexer micheline_parser.
+Require untyped_syntax micheline2michelson typer.
 
-Definition lex_and_parse_micheline (fuel : nat) (input : string)
-  : error.M micheline_syntax.micheline :=
+
+
+Definition get_contract_type (_ : syntax.contract_constant) :=
+  error.Failed syntax.type error.Typing.
+
+Definition lex_and_parse_micheline (fuel : nat) (input : string) :
+  error.M (micheline_syntax.loc_micheline) :=
   error.bind
     (fun s =>
        match micheline_parser.file fuel s with
@@ -14,3 +20,9 @@ Definition lex_and_parse_micheline (fuel : nat) (input : string)
          error.Return _ m
        end)
     (micheline_lexer.lex_micheline_to_parser input).
+
+Definition lex_and_parse_and_expand_type (fuel : nat) (input : string)
+  : error.M syntax.type :=
+  error.bind
+    (fun m => micheline2michelson.micheline2michelson_type m)
+    (lex_and_parse_micheline fuel input).
