src/michocoq/location.v
@@ -1,0 +1,19 @@
+Require Import Arith.
+
+Record location := Mk_loc { line : nat; column : nat }.
+
+Lemma location_dec (x y : location) : {x = y} + {x <> y}.
+Proof.
+  decide equality; apply Nat.eq_dec.
+Qed.
+
+Definition location_add (loc : location) (n : nat) : location :=
+  {| line := loc.(line); column := n + loc.(column) |}.
+
+Definition location_start : location :=
+  {| line := 0; column := 0 |}.
+
+Definition location_incr (loc : location) := location_add loc 1.
+
+Definition location_newline (loc : location) : location :=
+  {| line := S (loc.(line)); column := 0 |}.
