src/michocoq/micheline_syntax.v
@@ -1,8 +1,14 @@
 Require Import String ZArith.
+Require Import location.
 
-Inductive micheline :=
-| SEQ (_ : list micheline)
-| PRIM (_ : string) (_ : list micheline)
+Inductive micheline : Set :=
+| SEQ (_ : list loc_micheline)
+| PRIM (_ : location * location * string)
+       (_ : list loc_micheline)
 | STR (_ : string)
 | BYTES (_ : string)
-| NUMBER (_ : Z).
+| NUMBER (_ : Z)
+with
+loc_micheline : Set :=
+| Mk_loc_micheline : location * location * micheline -> loc_micheline.
+
