src/michocoq/micheline_tokens.v
@@ -1,6 +1,7 @@
 Require Import String ZArith.
 Require micheline_parser.
 Import micheline_parser.Aut.GramDefs.
+Require Import location.
 
 (** Tokens *)
 Inductive token :=
@@ -17,41 +18,42 @@ Inductive token :=
 
 Definition parser_token := micheline_parser.Aut.GramDefs.token.
 
-Definition token_from_parser (t : parser_token) : token :=
+Definition token_from_parser (t : parser_token) : (location * location * token) :=
   match t with
-  | existT _ LBRACE't tt => LBRACE
-  | existT _ RBRACE't tt => RBRACE
-  | existT _ SEMICOLON't tt => SEMICOLON
-  | existT _ LPAREN't tt => LPAREN
-  | existT _ RPAREN't tt => RPAREN
-  | existT _ PRIM't s => PRIM s
-  | existT _ STR't s => STR s
-  | existT _ NUMBER't n => NUMBER n
-  | existT _ BYTES't s => BYTES s
-  | existT _ EOF't tt => EOF
+  | existT _ LBRACE't (b, e) => (b, e, LBRACE)
+  | existT _ RBRACE't (b, e) => (b, e, RBRACE)
+  | existT _ SEMICOLON't (b, e) => (b, e, SEMICOLON)
+  | existT _ LPAREN't (b, e) => (b, e, LPAREN)
+  | existT _ RPAREN't (b, e) => (b, e, RPAREN)
+  | existT _ PRIM't ((b, e), s) => (b, e, PRIM s)
+  | existT _ STR't ((b, e), s) => (b, e, STR s)
+  | existT _ NUMBER't ((b, e), n) => (b, e, NUMBER n)
+  | existT _ BYTES't ((b, e), s) => (b, e, BYTES s)
+  | existT _ EOF't (b, e) => (b, e, EOF)
   end.
 
-Definition token_to_parser (t : token) : parser_token :=
+Definition token_to_parser (t : (location * location * token)) : parser_token :=
+  let '((b, e), t) := t in
   match t with
-  | LBRACE => existT _ LBRACE't tt
-  | RBRACE => existT _ RBRACE't tt
-  | SEMICOLON => existT _ SEMICOLON't tt
-  | LPAREN => existT _ LPAREN't tt
-  | RPAREN => existT _ RPAREN't tt
-  | PRIM s => existT _ PRIM't s
-  | STR s => existT _ STR't s
-  | NUMBER n => existT _ NUMBER't n
-  | BYTES s => existT _ BYTES't s
-  | EOF => existT _ EOF't tt
+  | LBRACE => existT _ LBRACE't (b, e)
+  | RBRACE => existT _ RBRACE't (b, e)
+  | SEMICOLON => existT _ SEMICOLON't (b, e)
+  | LPAREN => existT _ LPAREN't (b, e)
+  | RPAREN => existT _ RPAREN't (b, e)
+  | PRIM s => existT _ PRIM't (b, e, s)
+  | STR s => existT _ STR't (b, e, s)
+  | NUMBER n => existT _ NUMBER't (b, e, n)
+  | BYTES s => existT _ BYTES't (b, e, s)
+  | EOF => existT _ EOF't (b, e)
   end.
 
 Lemma token_to_parser_from_parser t : token_to_parser (token_from_parser t) = t.
 Proof.
   destruct t as (terminal, semantic).
-  destruct terminal; try reflexivity; destruct semantic; reflexivity.
+  destruct terminal; try reflexivity; destruct semantic as ((b, e), v); reflexivity.
 Qed.
 
 Lemma token_from_parser_to_parser t : token_from_parser (token_to_parser t) = t.
 Proof.
-  destruct t; reflexivity.
+  destruct t as ((b, e), t); destruct t; reflexivity.
 Qed.
