src/michocoq/typer.v
@@ -1,0 +1,615 @@
+Require Import ZArith List.
+Require Import syntax.
+Require Import untyped_syntax error.
+
+
+Lemma andb_and a b : (a && b)%bool <-> a /\ b.
+Proof.
+  split.
+  - apply Bool.andb_prop_elim.
+  - apply Bool.andb_prop_intro.
+Qed.
+
+Module Typer(ST: SelfType)(C:ContractContext).
+
+  Module syntax := Syntax ST C.
+  Import syntax. Import untyped_syntax.
+
+  Definition instruction := syntax.instruction.
+
+  Definition safe_instruction_cast {tff} A A' B B' :
+    instruction tff A B -> A = A' -> B = B' -> instruction tff A' B'.
+  Proof.
+    intros i [] [].
+    exact i.
+  Defined.
+
+  Definition instruction_cast {tff} A A' B B' i : M (instruction tff A' B') :=
+    match stype_dec A A', stype_dec B B' with
+    | left HA, left HB => Return _ (safe_instruction_cast A A' B B' i HA HB)
+    | _, _ => Failed _ Typing
+    end.
+
+  Definition instruction_cast_range {tff} A B B' (i : instruction tff A B)
+    : M (instruction tff A B') := instruction_cast A A B B' i.
+
+  Definition instruction_cast_domain {tff} A A' B (i : instruction tff A B)
+    : M (instruction tff A' B) := instruction_cast A A' B B i.
+
+  Inductive typer_result A : Set :=
+  | Inferred_type B : instruction false A B -> typer_result A
+  | Any_type : (forall B, instruction true A B) -> typer_result A.
+
+  Definition type_check_instruction
+             (type_instruction :
+                forall (i : untyped_syntax.instruction) A,
+                  M (typer_result A))
+             i A B : M {b : Datatypes.bool & instruction b A B} :=
+    bind (fun r1 =>
+            match r1 with
+            | Inferred_type _ B' i =>
+              bind (fun i =>
+                      Return _ (existT _ false i))
+                   (instruction_cast_range A B' B i)
+            | Any_type _ i => Return _ (existT _ true (i B))
+            end)
+         (type_instruction i A).
+
+  Definition type_check_instruction_no_tail_fail
+             (type_instruction :
+                forall (i : untyped_syntax.instruction) A,
+                  M (typer_result A))
+             i A B : M (instruction Datatypes.false A B) :=
+    bind (fun r1 =>
+            match r1 with
+            | Inferred_type _ B' i => instruction_cast_range A B' B i
+            | Any_type _ i => Failed _ Typing
+            end)
+         (type_instruction i A).
+
+  Definition assert_not_tail_fail A (r : typer_result A) :
+    M {B & instruction Datatypes.false A B} :=
+    match r with
+    | Inferred_type _ B i => Return _ (existT _ B i)
+    | Any_type _ _ => Failed _ Typing
+    end.
+
+  Definition type_instruction_no_tail_fail
+             (type_instruction :
+                forall (i : untyped_syntax.instruction) A,
+                  M (typer_result A))
+             i A : M {B & instruction Datatypes.false A B} :=
+    bind (assert_not_tail_fail A)
+         (type_instruction i A).
+
+  Definition type_branches
+             (type_instruction :
+                forall (i : untyped_syntax.instruction) A,
+                  M (typer_result A))
+             i1 i2 A1 A2 A
+             (IF_instr : forall B tffa tffb,
+                 instruction tffa A1 B ->
+                 instruction tffb A2 B ->
+                 instruction (tffa && tffb) A B)
+    : M (typer_result A) :=
+    bind (fun r1 =>
+            bind (fun r2 =>
+                    match r1, r2 with
+                    | Inferred_type _ B1 i1, Inferred_type _ B2 i2 =>
+                      bind (fun i2 =>
+                              Return _
+                                     (Inferred_type _ _
+                                                    (IF_instr B1 false false i1 i2)))
+                           (instruction_cast_range A2 B2 B1 i2)
+                    | Inferred_type _ B i1, Any_type _ i2 =>
+                      Return _ (Inferred_type _ _ (IF_instr B false true i1 (i2 B)))
+                    | Any_type _ i1, Inferred_type _ B i2 =>
+                      Return _ (Inferred_type _ _ (IF_instr B true false (i1 B) i2))
+                    | Any_type _ i1, Any_type _ i2 =>
+                      Return _ (Any_type _ (fun B =>
+                                              IF_instr B true true (i1 B) (i2 B)))
+                    end)
+                 (type_instruction i2 A2))
+         (type_instruction i1 A1).
+
+  Fixpoint type_data (d : concrete_data) {struct d}
+    : forall ty, M (syntax.concrete_data ty) :=
+    match d with
+    | Int_constant z =>
+      fun ty =>
+        match ty with
+        | Comparable_type int => Return _ (syntax.Int_constant z)
+        | _ => Failed _ Typing
+        end
+    | Nat_constant n =>
+      fun ty =>
+        match ty with
+        | Comparable_type nat => Return _ (syntax.Nat_constant n)
+        | Comparable_type int => Return _ (syntax.Int_constant (Z.of_N n))
+        | _ => Failed _ Typing
+        end
+    | String_constant s =>
+      fun ty =>
+        match ty with
+        | Comparable_type string => Return _ (syntax.String_constant s)
+        | _ => Failed _ Typing
+        end
+    | Mutez_constant m =>
+      fun ty =>
+        match ty with
+        | Comparable_type mutez => Return _ (syntax.Mutez_constant m)
+        | _ => Failed _ Typing
+        end
+    | Bytes_constant s =>
+      fun ty =>
+        match ty with
+        | Comparable_type bytes => Return _ (syntax.Bytes_constant s)
+        | _ => Failed _ Typing
+        end
+    | Timestamp_constant s =>
+      fun ty =>
+        match ty with
+        | Comparable_type timestamp => Return _ (syntax.Timestamp_constant s)
+        | _ => Failed _ Typing
+        end
+    | Signature_constant s =>
+      fun ty =>
+        match ty with
+        | signature => Return _ (syntax.Signature_constant s)
+        | _ => Failed _ Typing
+        end
+    | Key_constant s =>
+      fun ty =>
+        match ty with
+        | key => Return _ (syntax.Key_constant s)
+        | _ => Failed _ Typing
+        end
+    | Key_hash_constant s =>
+      fun ty =>
+        match ty with
+        | Comparable_type key_hash => Return _ (syntax.Key_hash_constant s)
+        | _ => Failed _ Typing
+        end
+    | Contract_constant c =>
+      fun ty =>
+        match ty with
+        | contract a =>
+          match (mtype_dec (C.get_contract_type c) (Return _ a)) with
+          | left H => Return _ (syntax.Contract_constant c H)
+          | _ => Failed _ Typing
+          end
+        | _ => Failed _ Typing
+        end
+    | Unit =>
+      fun ty =>
+        match ty with
+        | unit => Return _ syntax.Unit
+        | _ => Failed _ Typing
+        end
+    | True_ =>
+      fun ty =>
+        match ty with
+        | Comparable_type bool => Return _ syntax.True_
+        | _ => Failed _ Typing
+        end
+    | False_ =>
+      fun ty =>
+        match ty with
+        | Comparable_type bool => Return _ syntax.False_
+        | _ => Failed _ Typing
+        end
+    | Pair x y =>
+      fun ty =>
+        match ty with
+        | pair a b =>
+          bind (fun x =>
+                  bind (fun y =>
+                          Return _ (syntax.Pair x y))
+                       (type_data y b))
+               (type_data x a)
+        | _ => Failed _ Typing
+        end
+    | Left x =>
+      fun ty =>
+        match ty with
+        | or a b =>
+          bind (fun x =>
+                  Return _ (syntax.Left x))
+               (type_data x a)
+        | _ => Failed _ Typing
+        end
+    | Right y =>
+      fun ty =>
+        match ty with
+        | or a b =>
+          bind (fun y =>
+                  Return _ (syntax.Right y))
+               (type_data y b)
+        | _ => Failed _ Typing
+        end
+    | Some_ x =>
+      fun ty =>
+        match ty with
+        | option a =>
+          bind (fun x =>
+                  Return _ (syntax.Some_ x))
+               (type_data x a)
+        | _ => Failed _ Typing
+        end
+    | None_ =>
+      fun ty =>
+        match ty with
+        | option a => Return _ syntax.None_
+        | _ => Failed _ Typing
+        end
+    | Concrete_seq l =>
+      fun ty =>
+        match ty with
+        | list a =>
+          bind (fun l => Return _ (syntax.Concrete_list l))
+               ((fix type_data_list l :=
+                   match l with
+                   | nil => Return _ nil
+                   | cons x l =>
+                     bind (fun x =>
+                             bind (fun l =>
+                                     Return _ (cons x l))
+                                  (type_data_list l))
+                          (type_data x a)
+                   end) l)
+        | set a =>
+          bind (fun l => Return _ (syntax.Concrete_set l))
+               ((fix type_data_list l :=
+                   match l with
+                   | nil => Return _ nil
+                   | cons x l =>
+                     bind (fun x =>
+                             bind (fun l =>
+                                     Return _ (cons x l))
+                                  (type_data_list l))
+                          (type_data x a)
+                   end) l)
+        | map a b =>
+          bind (fun l => Return _ (syntax.Concrete_map l))
+               ((fix type_data_list l :=
+                   match l with
+                   | nil => Return _ nil
+                   | cons (Elt x y) l =>
+                     bind (fun x =>
+                             bind (fun y =>
+                                     bind (fun l =>
+                                             Return _ (cons (syntax.Elt _ _ x y) l))
+                                          (type_data_list l))
+                                  (type_data y b))
+                          (type_data x a)
+                   | _ => Failed _ Typing
+                   end) l)
+        | _ => Failed _ Typing
+        end
+    | Instruction i =>
+      fun ty =>
+        match ty with
+        | syntax.lambda a b =>
+          bind
+            (fun '(existT _ tff i) => Return _ (syntax.Instruction _ i))
+            (type_check_instruction type_instruction i (cons a nil) (cons b nil))
+        | _ => Failed _ Typing
+        end
+    | _ => fun _ => Failed _ Typing
+    end
+
+  with
+  type_instruction i A {struct i} : M (typer_result A) :=
+    match i, A with
+    | NOOP, A => Return _ (Inferred_type _ _ syntax.NOOP)
+    | FAILWITH, a :: A => Return _ (Any_type _ (fun B => syntax.FAILWITH))
+    | SEQ i1 i2, A =>
+      bind (fun '(existT _ B i1) =>
+              bind (fun r2 =>
+                      match r2 with
+                      | Inferred_type _ C i2 =>
+                        Return _ (Inferred_type _ _ (syntax.SEQ i1 i2))
+                      | Any_type _ i2 =>
+                        Return _ (Any_type _ (fun C => syntax.SEQ i1 (i2 C)))
+                      end)
+                   (type_instruction i2 B))
+           (type_instruction_no_tail_fail type_instruction i1 A)
+    | IF_ i1 i2, Comparable_type bool :: A =>
+      type_branches type_instruction i1 i2 _ _ _ (fun B tffa tffb => syntax.IF_)
+    | IF_NONE i1 i2, option a :: A =>
+      type_branches type_instruction i1 i2 _ _ _ (fun B tffa tffb => syntax.IF_NONE)
+    | IF_LEFT i1 i2, or a b :: A =>
+      type_branches type_instruction i1 i2 _ _ _ (fun B tffa tffb => syntax.IF_LEFT)
+    | IF_RIGHT i1 i2, or a b :: A =>
+      type_branches type_instruction i1 i2 _ _ _ (fun B tffa tffb => syntax.IF_RIGHT)
+    | IF_CONS i1 i2, list a :: A =>
+      type_branches type_instruction i1 i2 _ _ _ (fun B tffa tffb => syntax.IF_CONS)
+    | LOOP i, Comparable_type bool :: A =>
+      bind (fun i => Return _ (Inferred_type _ _ (syntax.LOOP i)))
+           (type_check_instruction_no_tail_fail
+              type_instruction i A (bool ::: A))
+    | LOOP_LEFT i, syntax.or a b :: A =>
+      bind (fun i => Return _ (Inferred_type _ _ (syntax.LOOP_LEFT i)))
+           (type_check_instruction_no_tail_fail
+              type_instruction i (a :: A) (syntax.or a b :: A))
+    | EXEC, a :: lambda a' b :: B =>
+      let A := a :: lambda a' b :: B in
+      let A' := a :: lambda a b :: B in
+      bind (fun i => Return _ (Inferred_type _ _ i))
+           (instruction_cast_domain A' A _ syntax.EXEC)
+    | DUP, a :: A =>
+      Return _ (Inferred_type _ _ syntax.DUP)
+    | SWAP, a :: b :: A =>
+      Return _ (Inferred_type _ _ syntax.SWAP)
+    | PUSH a v, A =>
+      bind (fun d => Return _ (Inferred_type _ _ (syntax.PUSH a d)))
+           (type_data v a)
+    | UNIT, A => Return _ (Inferred_type _ _ syntax.UNIT)
+    | LAMBDA a b i, A =>
+      bind (fun '(existT _ tff i) =>
+              Return _ (Inferred_type _ _ (syntax.LAMBDA a b i)))
+           (type_check_instruction
+              type_instruction i (a :: nil) (b :: nil))
+    | EQ, Comparable_type int :: A =>
+      Return _ (Inferred_type _ _ syntax.EQ)
+    | NEQ, Comparable_type int :: A =>
+      Return _ (Inferred_type _ _ syntax.NEQ)
+    | LT, Comparable_type int :: A =>
+      Return _ (Inferred_type _ _ syntax.LT)
+    | GT, Comparable_type int :: A =>
+      Return _ (Inferred_type _ _ syntax.GT)
+    | LE, Comparable_type int :: A =>
+      Return _ (Inferred_type _ _ syntax.LE)
+    | GE, Comparable_type int :: A =>
+      Return _ (Inferred_type _ _ syntax.GE)
+    | OR, Comparable_type bool :: Comparable_type bool :: A =>
+      Return _ (Inferred_type _ _ (@syntax.OR _ syntax.bitwise_bool _))
+    | OR, Comparable_type nat :: Comparable_type nat :: A =>
+      Return _ (Inferred_type _ _ (@syntax.OR _ syntax.bitwise_nat _))
+    | AND, Comparable_type bool :: Comparable_type bool :: A =>
+      Return _ (Inferred_type _ _ (@syntax.AND _ syntax.bitwise_bool _))
+    | AND, Comparable_type nat :: Comparable_type nat :: A =>
+      Return _ (Inferred_type _ _ (@syntax.AND _ syntax.bitwise_nat _))
+    | XOR, Comparable_type bool :: Comparable_type bool :: A =>
+      Return _ (Inferred_type _ _ (@syntax.XOR _ syntax.bitwise_bool _))
+    | XOR, Comparable_type nat :: Comparable_type nat :: A =>
+      Return _ (Inferred_type _ _ (@syntax.XOR _ syntax.bitwise_nat _))
+    | NOT, Comparable_type bool :: A =>
+      Return _ (Inferred_type _ _ (@syntax.NOT _ syntax.not_bool _))
+    | NOT, Comparable_type nat :: A =>
+      Return _ (Inferred_type _ _ (@syntax.NOT _ syntax.not_nat _))
+    | NOT, Comparable_type int :: A =>
+      Return _ (Inferred_type _ _ (@syntax.NOT _ syntax.not_int _))
+    | NEG, Comparable_type nat :: A =>
+      Return _ (Inferred_type _ _ (@syntax.NEG _ syntax.neg_nat _))
+    | NEG, Comparable_type int :: A =>
+      Return _ (Inferred_type _ _ (@syntax.NEG _ syntax.neg_int _))
+    | ABS, Comparable_type int :: A =>
+      Return _ (Inferred_type _ _ syntax.ABS)
+    | ADD, Comparable_type nat :: Comparable_type nat :: A =>
+      Return _ (Inferred_type _ _ (@syntax.ADD _ _ syntax.add_nat_nat _))
+    | ADD, Comparable_type nat :: Comparable_type int :: A =>
+      Return _ (Inferred_type _ _ (@syntax.ADD _ _ syntax.add_nat_int _))
+    | ADD, Comparable_type int :: Comparable_type nat :: A =>
+      Return _ (Inferred_type _ _ (@syntax.ADD _ _ syntax.add_int_nat _))
+    | ADD, Comparable_type int :: Comparable_type int :: A =>
+      Return _ (Inferred_type _ _ (@syntax.ADD _ _ syntax.add_int_int _))
+    | ADD, Comparable_type timestamp :: Comparable_type int :: A =>
+      Return _ (Inferred_type _ _ (@syntax.ADD _ _ syntax.add_timestamp_int _))
+    | ADD, Comparable_type int :: Comparable_type timestamp :: A =>
+      Return _ (Inferred_type _ _ (@syntax.ADD _ _ syntax.add_int_timestamp _))
+    | ADD, Comparable_type mutez :: Comparable_type mutez :: A =>
+      Return _ (Inferred_type _ _ (@syntax.ADD _ _ syntax.add_tez_tez _))
+    | SUB, Comparable_type nat :: Comparable_type nat :: A =>
+      Return _ (Inferred_type _ _ (@syntax.SUB _ _ syntax.sub_nat_nat _))
+    | SUB, Comparable_type nat :: Comparable_type int :: A =>
+      Return _ (Inferred_type _ _ (@syntax.SUB _ _ syntax.sub_nat_int _))
+    | SUB, Comparable_type int :: Comparable_type nat :: A =>
+      Return _ (Inferred_type _ _ (@syntax.SUB _ _ syntax.sub_int_nat _))
+    | SUB, Comparable_type int :: Comparable_type int :: A =>
+      Return _ (Inferred_type _ _ (@syntax.SUB _ _ syntax.sub_int_int _))
+    | SUB, Comparable_type timestamp :: Comparable_type int :: A =>
+      Return _ (Inferred_type _ _ (@syntax.SUB _ _ syntax.sub_timestamp_int _))
+    | SUB, Comparable_type timestamp :: Comparable_type timestamp :: A =>
+      Return _ (Inferred_type _ _ (@syntax.SUB _ _ syntax.sub_timestamp_timestamp _))
+    | SUB, Comparable_type mutez :: Comparable_type mutez :: A =>
+      Return _ (Inferred_type _ _ (@syntax.SUB _ _ syntax.sub_tez_tez _))
+    | MUL, Comparable_type nat :: Comparable_type nat :: A =>
+      Return _ (Inferred_type _ _ (@syntax.MUL _ _ syntax.mul_nat_nat _))
+    | MUL, Comparable_type nat :: Comparable_type int :: A =>
+      Return _ (Inferred_type _ _ (@syntax.MUL _ _ syntax.mul_nat_int _))
+    | MUL, Comparable_type int :: Comparable_type nat :: A =>
+      Return _ (Inferred_type _ _ (@syntax.MUL _ _ syntax.mul_int_nat _))
+    | MUL, Comparable_type int :: Comparable_type int :: A =>
+      Return _ (Inferred_type _ _ (@syntax.MUL _ _ syntax.mul_int_int _))
+    | MUL, Comparable_type mutez :: Comparable_type nat :: A =>
+      Return _ (Inferred_type _ _ (@syntax.MUL _ _ syntax.mul_tez_nat _))
+    | MUL, Comparable_type nat :: Comparable_type mutez :: A =>
+      Return _ (Inferred_type _ _ (@syntax.MUL _ _ syntax.mul_nat_tez _))
+    | EDIV, Comparable_type nat :: Comparable_type nat :: A =>
+      Return _ (Inferred_type _ _ (@syntax.EDIV _ _ syntax.ediv_nat_nat _))
+    | EDIV, Comparable_type nat :: Comparable_type int :: A =>
+      Return _ (Inferred_type _ _ (@syntax.EDIV _ _ syntax.ediv_nat_int _))
+    | EDIV, Comparable_type int :: Comparable_type nat :: A =>
+      Return _ (Inferred_type _ _ (@syntax.EDIV _ _ syntax.ediv_int_nat _))
+    | EDIV, Comparable_type int :: Comparable_type int :: A =>
+      Return _ (Inferred_type _ _ (@syntax.EDIV _ _ syntax.ediv_int_int _))
+    | EDIV, Comparable_type mutez :: Comparable_type nat :: A =>
+      Return _ (Inferred_type _ _ (@syntax.EDIV _ _ syntax.ediv_tez_nat _))
+    | EDIV, Comparable_type mutez :: Comparable_type mutez :: A =>
+      Return _ (Inferred_type _ _ (@syntax.EDIV _ _ syntax.ediv_tez_tez _))
+    | LSL, Comparable_type nat :: Comparable_type nat :: A =>
+      Return _ (Inferred_type _ _ syntax.LSL)
+    | LSR, Comparable_type nat :: Comparable_type nat :: A =>
+      Return _ (Inferred_type _ _ syntax.LSR)
+    | COMPARE, Comparable_type a :: Comparable_type a' :: B =>
+      let A := a ::: a' ::: B in
+      let A' := a ::: a ::: B in
+      bind (fun i => Return _ (Inferred_type _ _ i))
+           (instruction_cast_domain
+              A' A (int ::: B) syntax.COMPARE)
+    | CONCAT, Comparable_type string :: Comparable_type string :: B =>
+      Return _ (Inferred_type _ _ (@syntax.CONCAT _ stringlike_string _))
+    | CONCAT, Comparable_type bytes :: Comparable_type bytes :: B =>
+      Return _ (Inferred_type _ _ (@syntax.CONCAT _ stringlike_bytes _))
+    | SIZE, set a :: A =>
+      Return _ (Inferred_type _ _ (@syntax.SIZE _ (size_set a) _))
+    | SIZE, cons (list a) A =>
+      Return _ (Inferred_type _ _ (@syntax.SIZE _ (size_list a) _))
+    | SIZE, cons (map a b) A =>
+      Return _ (Inferred_type _ _ (@syntax.SIZE _ (size_map a b) _))
+    | SIZE, Comparable_type string :: A =>
+      Return _ (Inferred_type _ _ (@syntax.SIZE _ size_string _))
+    | SIZE, Comparable_type bytes :: A =>
+      Return _ (Inferred_type _ _ (@syntax.SIZE _ size_bytes _))
+    | SLICE, Comparable_type nat :: Comparable_type nat :: Comparable_type string :: A =>
+      Return _ (Inferred_type _ _ (@syntax.SLICE _ stringlike_string _))
+    | SLICE, Comparable_type nat :: Comparable_type nat :: Comparable_type bytes :: A =>
+      Return _ (Inferred_type _ _ (@syntax.SLICE _ stringlike_bytes _))
+    | PAIR, a :: b :: A =>
+      Return _ (Inferred_type _ _ syntax.PAIR)
+    | CAR, pair a b :: A =>
+      Return _ (Inferred_type _ _ syntax.CAR)
+    | CDR, pair a b :: A =>
+      Return _ (Inferred_type _ _ syntax.CDR)
+    | EMPTY_SET c, A =>
+      Return _ (Inferred_type _ _ (syntax.EMPTY_SET c))
+    | MEM, elt' :: set elt :: B =>
+      let A := elt' :: set elt :: B in
+      let A' := elt ::: set elt :: B in
+      bind (fun i => Return _ (Inferred_type _ _ i))
+           (instruction_cast_domain
+              A' A _ (@syntax.MEM _ _ (mem_set elt) _))
+    | MEM, kty' :: map kty vty :: B =>
+      let A := kty' :: map kty vty :: B in
+      let A' := kty ::: map kty vty :: B in
+      bind (fun i => Return _ (Inferred_type _ _ i))
+           (instruction_cast_domain
+              A' A _ (@syntax.MEM _ _ (mem_map kty vty) _))
+    | MEM, kty' :: big_map kty vty :: B =>
+      let A := kty' :: big_map kty vty :: B in
+      let A' := kty ::: big_map kty vty :: B in
+      bind (fun i => Return _ (Inferred_type _ _ i))
+           (instruction_cast_domain
+              A' A _ (@syntax.MEM _ _ (mem_bigmap kty vty) _))
+    | UPDATE, elt' :: Comparable_type bool :: set elt :: B =>
+      let A := elt' ::: bool ::: set elt :: B in
+      let A' := elt ::: bool ::: set elt :: B in
+      bind (fun i => Return _ (Inferred_type _ _ i))
+           (instruction_cast_domain
+              A' A _ (@syntax.UPDATE _ _ _ (update_set elt) _))
+    | UPDATE, kty' :: option vty' :: map kty vty :: B =>
+      let A := kty' ::: option vty' ::: map kty vty :: B in
+      let A' := kty ::: option vty ::: map kty vty :: B in
+      bind (fun i => Return _ (Inferred_type _ _ i))
+           (instruction_cast_domain
+              A' A _ (@syntax.UPDATE _ _ _ (update_map kty vty) _))
+    | UPDATE, kty' :: option vty' :: big_map kty vty :: B =>
+      let A := kty' ::: option vty' ::: big_map kty vty :: B in
+      let A' := kty ::: option vty ::: big_map kty vty :: B in
+      bind (fun i => Return _ (Inferred_type _ _ i))
+           (instruction_cast_domain
+              A' A _ (@syntax.UPDATE _ _ _ (update_bigmap kty vty) _))
+    | ITER i, list a :: A =>
+      bind (fun i => Return _ (Inferred_type _ _ (syntax.ITER i)))
+           (type_check_instruction_no_tail_fail type_instruction i (a :: A) A)
+    | ITER i, set a :: A =>
+      bind (fun i => Return _ (Inferred_type _ _ (syntax.ITER i)))
+           (type_check_instruction_no_tail_fail type_instruction i (a ::: A) A)
+    | ITER i, map kty vty :: A =>
+      bind (fun i => Return _ (Inferred_type _ _ (syntax.ITER i)))
+           (type_check_instruction_no_tail_fail type_instruction i (pair kty vty :: A) A)
+    | EMPTY_MAP kty vty, A =>
+      Return _ (Inferred_type _ _ (syntax.EMPTY_MAP kty vty))
+    | GET, kty' :: map kty vty :: B =>
+      let A := kty' :: map kty vty :: B in
+      let A' := kty ::: map kty vty :: B in
+      bind (fun i => Return _ (Inferred_type _ _ i))
+           (instruction_cast_domain
+              A' A _ (@syntax.GET _ _ (get_map kty vty) _))
+    | GET, kty' :: big_map kty vty :: B =>
+      let A := kty' :: big_map kty vty :: B in
+      let A' := kty ::: big_map kty vty :: B in
+      bind (fun i => Return _ (Inferred_type _ _ i))
+           (instruction_cast_domain
+              A' A _ (@syntax.GET _ _ (get_bigmap kty vty) _))
+    | MAP i, list a :: A =>
+      bind (fun r =>
+              match r with
+              | existT _ (b :: A') i =>
+                bind (fun i => Return _ (Inferred_type _ _ (syntax.MAP i)))
+                     (instruction_cast_range (a :: A) (b :: A') (b :: A) i)
+              | _ => Failed _ Typing
+              end)
+           (type_instruction_no_tail_fail type_instruction i (a :: A))
+    | MAP i, map kty vty :: A =>
+      bind (fun r =>
+              match r with
+              | existT _ (b :: A') i =>
+                bind (fun i => Return _ (Inferred_type _ _ (syntax.MAP i)))
+                     (instruction_cast_range (pair kty vty :: A) (b :: A') (b :: A) i)
+              | _ => Failed _ Typing
+              end)
+           (type_instruction_no_tail_fail type_instruction i (pair kty vty ::: A))
+    | SOME, a :: A => Return _ (Inferred_type _ _ syntax.SOME)
+    | NONE a, A => Return _ (Inferred_type _ _ (syntax.NONE a))
+    | LEFT b, a :: A => Return _ (Inferred_type _ _ (syntax.LEFT b))
+    | RIGHT a, b :: A => Return _ (Inferred_type _ _ (syntax.RIGHT a))
+    | CONS, a' :: list a :: B =>
+      let A := a' :: list a :: B in
+      let A' := a :: list a :: B in
+      bind (fun i => Return _ (Inferred_type _ _ i))
+           (instruction_cast_domain A' A _ (syntax.CONS))
+    | NIL a, A => Return _ (Inferred_type _ _ (syntax.NIL a))
+    | CREATE_CONTRACT g p i,
+      option (Comparable_type key_hash) :: Comparable_type mutez :: g2 :: B =>
+      let A :=
+          option key_hash ::: mutez ::: g2 :: B in
+      let A' :=
+          option key_hash ::: mutez ::: g ::: B in
+      bind (fun '(existT _ tff i) =>
+              bind (fun i => Return _ (Inferred_type _ _ i))
+                   (instruction_cast_domain A' A _ (syntax.CREATE_CONTRACT g p i)))
+           (type_check_instruction type_instruction i (pair p g :: nil) (pair (list operation) g :: nil))
+    | TRANSFER_TOKENS, p1 :: Comparable_type mutez :: contract p2 :: B =>
+      let A := p1 ::: mutez ::: contract p2 ::: B in
+      let A' := p1 ::: mutez ::: contract p1 ::: B in
+      bind (fun i => Return _ (Inferred_type _ _ i))
+           (instruction_cast_domain A' A _ syntax.TRANSFER_TOKENS)
+    | SET_DELEGATE, option (Comparable_type key_hash) :: A =>
+      Return _ (Inferred_type _ _ syntax.SET_DELEGATE)
+    | BALANCE, A =>
+      Return _ (Inferred_type _ _ syntax.BALANCE)
+    | ADDRESS, contract _ :: A =>
+      Return _ (Inferred_type _ _ syntax.ADDRESS)
+    | CONTRACT ty, Comparable_type address :: A =>
+      Return _ (Inferred_type _ _ (syntax.CONTRACT ty))
+    | SOURCE, A =>
+      Return _ (Inferred_type _ _ syntax.SOURCE)
+    | SENDER, A =>
+      Return _ (Inferred_type _ _ syntax.SENDER)
+    | SELF, A =>
+      Return _ (Inferred_type _ _ syntax.SELF)
+    | AMOUNT, A =>
+      Return _ (Inferred_type _ _ syntax.AMOUNT)
+    | IMPLICIT_ACCOUNT, Comparable_type key_hash :: A =>
+      Return _ (Inferred_type _ _ syntax.IMPLICIT_ACCOUNT)
+    | NOW, A =>
+      Return _ (Inferred_type _ _ syntax.NOW)
+    | PACK, a :: A =>
+      Return _ (Inferred_type _ _ syntax.PACK)
+    | UNPACK ty, Comparable_type bytes :: A =>
+      Return _ (Inferred_type _ _ (syntax.UNPACK ty))
+    | HASH_KEY, key :: A =>
+      Return _ (Inferred_type _ _ syntax.HASH_KEY)
+    | BLAKE2B, Comparable_type bytes :: A =>
+      Return _ (Inferred_type _ _ syntax.BLAKE2B)
+    | SHA256, Comparable_type bytes :: A =>
+      Return _ (Inferred_type _ _ syntax.SHA256)
+    | SHA512, Comparable_type bytes :: A =>
+      Return _ (Inferred_type _ _ syntax.SHA512)
+    | CHECK_SIGNATURE, key :: signature :: Comparable_type bytes :: A =>
+      Return _ (Inferred_type _ _ syntax.CHECK_SIGNATURE)
+    | _, _ => Failed _ Typing
+    end.
+End Typer.
