src/michocoq/untyped_syntax.v
@@ -1,0 +1,114 @@
+Require syntax.
+Require Import ZArith String.
+
+Definition type := syntax.type.
+Definition comparable_type := syntax.comparable_type.
+
+
+Inductive instruction : Set :=
+| NOOP : instruction
+| FAILWITH : instruction
+| SEQ : instruction -> instruction -> instruction
+| IF_ : instruction -> instruction -> instruction
+| LOOP : instruction -> instruction
+| LOOP_LEFT : instruction -> instruction
+| EXEC : instruction
+| APPLY : instruction
+| DUP : instruction
+| SWAP : instruction
+| PUSH : syntax.type -> concrete_data -> instruction
+| UNIT : instruction
+| LAMBDA : syntax.type -> syntax.type -> instruction -> instruction
+| EQ : instruction
+| NEQ : instruction
+| LT : instruction
+| GT : instruction
+| LE : instruction
+| GE : instruction
+| OR : instruction
+| AND : instruction
+| XOR : instruction
+| NOT : instruction
+| NEG : instruction
+| ABS : instruction
+| INT : instruction
+| ISNAT : instruction
+| ADD : instruction
+| SUB : instruction
+| MUL : instruction
+| EDIV : instruction
+| LSL : instruction
+| LSR : instruction
+| COMPARE : instruction
+| CONCAT : instruction
+| SIZE : instruction
+| SLICE : instruction
+| PAIR : instruction
+| CAR : instruction
+| CDR : instruction
+| EMPTY_SET : comparable_type -> instruction
+| MEM : instruction
+| UPDATE : instruction
+| ITER : instruction -> instruction
+| EMPTY_MAP : comparable_type -> type -> instruction
+| GET : instruction
+| MAP : instruction -> instruction
+| SOME : instruction
+| NONE : type -> instruction
+| IF_NONE : instruction -> instruction -> instruction
+| LEFT : type -> instruction
+| RIGHT : type -> instruction
+| IF_LEFT : instruction -> instruction -> instruction
+| IF_RIGHT : instruction -> instruction -> instruction
+| CONS : instruction
+| NIL : type -> instruction
+| IF_CONS : instruction -> instruction -> instruction
+| CREATE_CONTRACT : type -> type -> instruction -> instruction
+| TRANSFER_TOKENS : instruction
+| SET_DELEGATE : instruction
+| BALANCE : instruction
+| ADDRESS : instruction
+| CONTRACT : type -> instruction
+| SOURCE : instruction
+| SENDER : instruction
+| SELF : instruction
+| AMOUNT : instruction
+| IMPLICIT_ACCOUNT : instruction
+| NOW : instruction
+| PACK : instruction
+| UNPACK : type -> instruction
+| HASH_KEY : instruction
+| BLAKE2B : instruction
+| SHA256 : instruction
+| SHA512 : instruction
+| CHECK_SIGNATURE : instruction
+| DIG : Datatypes.nat -> instruction
+| DUG : Datatypes.nat -> instruction
+| DIP : Datatypes.nat -> instruction -> instruction
+| DROP : Datatypes.nat -> instruction
+| CHAIN_ID : instruction
+with
+concrete_data : Set :=
+| Int_constant : Z -> concrete_data
+| Nat_constant : N -> concrete_data
+| String_constant : String.string -> concrete_data
+| Mutez_constant : syntax.mutez_constant -> concrete_data
+| Bytes_constant : String.string -> concrete_data
+| Timestamp_constant : Z -> concrete_data
+| Signature_constant : String.string -> concrete_data
+| Key_constant : String.string -> concrete_data
+| Key_hash_constant : String.string -> concrete_data
+| Contract_constant : syntax.contract_constant -> concrete_data
+| Address_constant : syntax.address_constant -> concrete_data
+| Unit : concrete_data
+| True_ : concrete_data
+| False_ : concrete_data
+| Pair : concrete_data -> concrete_data -> concrete_data
+| Left : concrete_data -> concrete_data
+| Right : concrete_data -> concrete_data
+| Some_ : concrete_data -> concrete_data
+| None_ : concrete_data
+| Elt : concrete_data -> concrete_data -> concrete_data
+| Concrete_seq : Datatypes.list concrete_data -> concrete_data
+| Instruction : instruction -> concrete_data
+| Chain_id_constant : syntax.chain_id_constant -> concrete_data.
