src/michocoq/untyper.v
@@ -1,0 +1,811 @@
+Require Import ZArith List.
+Require Import syntax.
+Require Import untyped_syntax error.
+Require typer.
+Require Eqdep_dec.
+
+Module untyper(ST: SelfType)(C:ContractContext).
+
+  Module syntax := Syntax ST C.
+  Module typer := typer.Typer ST C.
+  Import typer. Import syntax. Import untyped_syntax.
+
+
+  Fixpoint untype_data {a} (d : syntax.concrete_data a) : concrete_data :=
+    match d with
+    | syntax.Int_constant z => Int_constant z
+    | syntax.Nat_constant n => Nat_constant n
+    | syntax.String_constant s => String_constant s
+    | syntax.Mutez_constant m => Mutez_constant m
+    | syntax.Bytes_constant s => Bytes_constant s
+    | syntax.Timestamp_constant t => Timestamp_constant t
+    | syntax.Signature_constant s => Signature_constant s
+    | syntax.Key_constant s => Key_constant s
+    | syntax.Key_hash_constant s => Key_hash_constant s
+    | syntax.Contract_constant c _ => Contract_constant c
+    | syntax.Address_constant c => Address_constant c
+    | syntax.Unit => Unit
+    | syntax.True_ => True_
+    | syntax.False_ => False_
+    | syntax.Pair x y => Pair (untype_data x) (untype_data y)
+    | syntax.Left x => Left (untype_data x)
+    | syntax.Right y => Right (untype_data y)
+    | syntax.Some_ x => Some_ (untype_data x)
+    | syntax.None_ => None_
+    | syntax.Concrete_list l => Concrete_seq (List.map (fun x => untype_data x) l)
+    | syntax.Concrete_set l => Concrete_seq (List.map (fun x => untype_data x) l)
+    | syntax.Concrete_map l =>
+      Concrete_seq (List.map
+                      (fun '(syntax.Elt _ _ x y) => Elt (untype_data x) (untype_data y))
+                      l)
+    | syntax.Instruction _ i => Instruction (untype_instruction i)
+    | syntax.Chain_id_constant c => Chain_id_constant c
+    end
+  with
+  untype_instruction {tff0 A B} (i : syntax.instruction tff0 A B) : instruction :=
+    match i with
+    | syntax.NOOP => NOOP
+    | syntax.FAILWITH => FAILWITH
+    | syntax.SEQ i1 i2 => SEQ (untype_instruction i1) (untype_instruction i2)
+    | syntax.IF_ i1 i2 => IF_ (untype_instruction i1) (untype_instruction i2)
+    | syntax.LOOP i => LOOP (untype_instruction i)
+    | syntax.LOOP_LEFT i => LOOP_LEFT (untype_instruction i)
+    | syntax.DIP n _ i => DIP n (untype_instruction i)
+    | syntax.EXEC => EXEC
+    | syntax.APPLY => APPLY
+    | syntax.DROP n _ => DROP n
+    | syntax.DUP => DUP
+    | syntax.SWAP => SWAP
+    | syntax.PUSH a x => PUSH a (untype_data x)
+    | syntax.UNIT => UNIT
+    | syntax.LAMBDA a b i => LAMBDA a b (untype_instruction i)
+    | syntax.EQ => EQ
+    | syntax.NEQ => NEQ
+    | syntax.LT => LT
+    | syntax.GT => GT
+    | syntax.LE => LE
+    | syntax.GE => GE
+    | syntax.OR => OR
+    | syntax.AND => AND
+    | syntax.XOR => XOR
+    | syntax.NOT => NOT
+    | syntax.NEG => NEG
+    | syntax.ABS => ABS
+    | syntax.INT => INT
+    | syntax.ISNAT => ISNAT
+    | syntax.ADD => ADD
+    | syntax.SUB => SUB
+    | syntax.MUL => MUL
+    | syntax.EDIV => EDIV
+    | syntax.LSL => LSL
+    | syntax.LSR => LSR
+    | syntax.COMPARE => COMPARE
+    | syntax.CONCAT => CONCAT
+    | syntax.SIZE => SIZE
+    | syntax.SLICE => SLICE
+    | syntax.PAIR => PAIR
+    | syntax.CAR => CAR
+    | syntax.CDR => CDR
+    | syntax.EMPTY_SET a => EMPTY_SET a
+    | syntax.MEM => MEM
+    | syntax.UPDATE => UPDATE
+    | syntax.ITER i => ITER (untype_instruction i)
+    | syntax.EMPTY_MAP kty vty => EMPTY_MAP kty vty
+    | syntax.GET => GET
+    | syntax.MAP i => MAP (untype_instruction i)
+    | syntax.SOME => SOME
+    | syntax.NONE a => NONE a
+    | syntax.IF_NONE i1 i2 => IF_NONE (untype_instruction i1) (untype_instruction i2)
+    | syntax.LEFT b => LEFT b
+    | syntax.RIGHT a => RIGHT a
+    | syntax.IF_LEFT i1 i2 => IF_LEFT (untype_instruction i1) (untype_instruction i2)
+    | syntax.IF_RIGHT i1 i2 => IF_RIGHT (untype_instruction i1) (untype_instruction i2)
+    | syntax.CONS => CONS
+    | syntax.NIL a => NIL a
+    | syntax.IF_CONS i1 i2 => IF_CONS (untype_instruction i1) (untype_instruction i2)
+    | syntax.CREATE_CONTRACT g p i => CREATE_CONTRACT g p (untype_instruction i)
+    | syntax.TRANSFER_TOKENS => TRANSFER_TOKENS
+    | syntax.SET_DELEGATE => SET_DELEGATE
+    | syntax.BALANCE => BALANCE
+    | syntax.ADDRESS => ADDRESS
+    | syntax.CONTRACT a => CONTRACT a
+    | syntax.SOURCE => SOURCE
+    | syntax.SENDER => SENDER
+    | syntax.SELF => SELF
+    | syntax.AMOUNT => AMOUNT
+    | syntax.IMPLICIT_ACCOUNT => IMPLICIT_ACCOUNT
+    | syntax.NOW => NOW
+    | syntax.PACK => PACK
+    | syntax.UNPACK a => UNPACK a
+    | syntax.HASH_KEY => HASH_KEY
+    | syntax.BLAKE2B => BLAKE2B
+    | syntax.SHA256 => SHA256
+    | syntax.SHA512 => SHA512
+    | syntax.CHECK_SIGNATURE => CHECK_SIGNATURE
+    | syntax.DIG n _ => DIG n
+    | syntax.DUG n _ => DUG n
+    | syntax.CHAIN_ID => CHAIN_ID
+    end.
+
+  Lemma stype_dec_same A : stype_dec A A = left eq_refl.
+  Proof.
+    destruct (stype_dec A A) as [e | n].
+    - f_equal.
+      apply Eqdep_dec.UIP_dec.
+      apply stype_dec.
+    - destruct (n eq_refl).
+  Qed.
+
+  Lemma bool_dec_same (a : Datatypes.bool) (H : a = a) : H = eq_refl.
+  Proof.
+    apply Eqdep_dec.UIP_dec.
+    apply Bool.bool_dec.
+  Qed.
+
+  Fixpoint tail_fail_induction A B (i : syntax.instruction true A B)
+        (P : forall A B, syntax.instruction true A B -> Type)
+        (HFAILWITH : forall a A B, P (a ::: A) B syntax.FAILWITH)
+        (HSEQ : forall A B C i1 i2,
+            P B C i2 ->
+            P A C (i1;; i2))
+        (HIF : forall A B i1 i2,
+            P A B i1 ->
+            P A B i2 ->
+            P (bool ::: A) B (syntax.IF_ i1 i2))
+        (HIF_NONE : forall a A B i1 i2,
+            P A B i1 ->
+            P (a ::: A) B i2 ->
+            P (option a ::: A) B (syntax.IF_NONE i1 i2))
+        (HIF_LEFT : forall a b A B i1 i2,
+            P (a ::: A) B i1 ->
+            P (b ::: A) B i2 ->
+            P (or a b ::: A) B (syntax.IF_LEFT i1 i2))
+        (HIF_RIGHT : forall a b A B i1 i2,
+            P (b ::: A) B i1 ->
+            P (a ::: A) B i2 ->
+            P (or a b ::: A) B (syntax.IF_RIGHT i1 i2))
+        (HIF_CONS : forall a A B i1 i2,
+            P (a ::: list a ::: A) B i1 ->
+            P A B i2 ->
+            P (list a ::: A) B (syntax.IF_CONS i1 i2))
+    : P A B i :=
+    let P' b A B : syntax.instruction b A B -> Type :=
+        if b return syntax.instruction b A B -> Type
+        then P A B
+        else fun i => True
+    in
+    match i as i0 in syntax.instruction b A B return P' b A B i0
+    with
+    | syntax.FAILWITH => HFAILWITH _ _ _
+    | @syntax.SEQ A B C tff i1 i2 =>
+      (if tff return
+          forall i2 : syntax.instruction tff B C,
+            P' tff A C (syntax.SEQ i1 i2)
+       then
+         fun i2 =>
+           HSEQ _ _ _ i1 i2
+                (tail_fail_induction B C i2 P HFAILWITH HSEQ HIF HIF_NONE HIF_LEFT HIF_RIGHT HIF_CONS)
+       else fun i2 => I)
+        i2
+    | @syntax.IF_ A B tffa tffb i1 i2 =>
+      (if tffa as tffa return
+          forall i1, P' (tffa && tffb)%bool _ _ (syntax.IF_ i1 i2)
+       then
+         fun i1 =>
+           (if tffb return
+               forall i2,
+                 P' tffb _ _ (syntax.IF_ i1 i2)
+            then
+              fun i2 =>
+                HIF _ _ i1 i2
+                    (tail_fail_induction _ _ i1 P HFAILWITH HSEQ HIF HIF_NONE HIF_LEFT HIF_RIGHT HIF_CONS)
+                    (tail_fail_induction _ _ i2 P HFAILWITH HSEQ HIF HIF_NONE HIF_LEFT HIF_RIGHT HIF_CONS)
+            else
+              fun _ => I) i2
+       else
+         fun _ => I) i1
+    | @syntax.IF_NONE a A B tffa tffb i1 i2 =>
+      (if tffa as tffa return
+          forall i1, P' (tffa && tffb)%bool _ _ (syntax.IF_NONE i1 i2)
+       then
+         fun i1 =>
+           (if tffb return
+               forall i2,
+                 P' tffb _ _ (syntax.IF_NONE i1 i2)
+            then
+              fun i2 =>
+                HIF_NONE _ _ _ i1 i2
+                    (tail_fail_induction _ _ i1 P HFAILWITH HSEQ HIF HIF_NONE HIF_LEFT HIF_RIGHT HIF_CONS)
+                    (tail_fail_induction _ _ i2 P HFAILWITH HSEQ HIF HIF_NONE HIF_LEFT HIF_RIGHT HIF_CONS)
+            else
+              fun _ => I) i2
+       else
+         fun _ => I) i1
+    | @syntax.IF_LEFT a b A B tffa tffb i1 i2 =>
+      (if tffa as tffa return
+          forall i1, P' (tffa && tffb)%bool _ _ (syntax.IF_LEFT i1 i2)
+       then
+         fun i1 =>
+           (if tffb return
+               forall i2,
+                 P' tffb _ _ (syntax.IF_LEFT i1 i2)
+            then
+              fun i2 =>
+                HIF_LEFT _ _ _ _ i1 i2
+                    (tail_fail_induction _ _ i1 P HFAILWITH HSEQ HIF HIF_NONE HIF_LEFT HIF_RIGHT HIF_CONS)
+                    (tail_fail_induction _ _ i2 P HFAILWITH HSEQ HIF HIF_NONE HIF_LEFT HIF_RIGHT HIF_CONS)
+            else
+              fun _ => I) i2
+       else
+         fun _ => I) i1
+    | @syntax.IF_RIGHT a b A B tffa tffb i1 i2 =>
+      (if tffa as tffa return
+          forall i1, P' (tffa && tffb)%bool _ _ (syntax.IF_RIGHT i1 i2)
+       then
+         fun i1 =>
+           (if tffb return
+               forall i2,
+                 P' tffb _ _ (syntax.IF_RIGHT i1 i2)
+            then
+              fun i2 =>
+                HIF_RIGHT _ _ _ _ i1 i2
+                    (tail_fail_induction _ _ i1 P HFAILWITH HSEQ HIF HIF_NONE HIF_LEFT HIF_RIGHT HIF_CONS)
+                    (tail_fail_induction _ _ i2 P HFAILWITH HSEQ HIF HIF_NONE HIF_LEFT HIF_RIGHT HIF_CONS)
+            else
+              fun _ => I) i2
+       else
+         fun _ => I) i1
+    | @syntax.IF_CONS a A B tffa tffb i1 i2 =>
+      (if tffa as tffa return
+          forall i1, P' (tffa && tffb)%bool _ _ (syntax.IF_CONS i1 i2)
+       then
+         fun i1 =>
+           (if tffb return
+               forall i2,
+                 P' tffb _ _ (syntax.IF_CONS i1 i2)
+            then
+              fun i2 =>
+                HIF_CONS _ _ _ i1 i2
+                    (tail_fail_induction _ _ i1 P HFAILWITH HSEQ HIF HIF_NONE HIF_LEFT HIF_RIGHT HIF_CONS)
+                    (tail_fail_induction _ _ i2 P HFAILWITH HSEQ HIF HIF_NONE HIF_LEFT HIF_RIGHT HIF_CONS)
+            else
+              fun _ => I) i2
+       else
+         fun _ => I) i1
+    | _ => I
+    end.
+
+  Lemma bool_dec_same2 (x y : Datatypes.bool) (H1 H2 : x = y) (HH1 HH2 : H1 = H2) : HH1 = HH2.
+  Proof.
+    apply Eqdep_dec.UIP_dec.
+    intros x2 y2.
+    left.
+    apply Eqdep_dec.UIP_dec.
+    apply Bool.bool_dec.
+  Qed.
+
+  Lemma bool_dec_same_same (x : Datatypes.bool) : bool_dec_same x eq_refl = eq_refl.
+  Proof.
+    apply bool_dec_same2.
+  Qed.
+
+  Lemma andb_prop_refl : andb_prop true true eq_refl = conj eq_refl eq_refl.
+  Proof.
+    destruct (andb_prop true true eq_refl).
+    f_equal; apply bool_dec_same.
+  Qed.
+
+  Definition tail_fail_change_range A B B' (i : syntax.instruction true A B) :
+    syntax.instruction true A B'.
+  Proof.
+    apply (tail_fail_induction A B i (fun A B i => syntax.instruction true A B')); clear A B i.
+    - intros a A _.
+      apply syntax.FAILWITH.
+    - intros A B C i1 _ i2.
+      apply (syntax.SEQ i1 i2).
+    - intros A B _ _ i1 i2.
+      apply (syntax.IF_ i1 i2).
+    - intros a A B _ _ i1 i2.
+      apply (syntax.IF_NONE i1 i2).
+    - intros a b A B _ _ i1 i2.
+      apply (syntax.IF_LEFT i1 i2).
+    - intros a b A B _ _ i1 i2.
+      apply (syntax.IF_RIGHT i1 i2).
+    - intros a A B _ _ i1 i2.
+      apply (syntax.IF_CONS i1 i2).
+  Defined.
+
+
+  Lemma tail_fail_change_range_same A B (i : syntax.instruction true A B) :
+    tail_fail_change_range A B B i = i.
+  Proof.
+    apply (tail_fail_induction A B i); clear A B i;
+      intros; unfold tail_fail_change_range; simpl; f_equal; assumption.
+  Qed.
+
+  Definition untype_type_spec tffi A B (i : syntax.instruction tffi A B) :=
+    typer.type_instruction (untype_instruction i) A =
+    Return _ ((if tffi return syntax.instruction tffi A B -> typer.typer_result A
+               then
+                 fun i =>
+                   typer.Any_type _ (fun B' => tail_fail_change_range A B B' i)
+               else
+                 typer.Inferred_type _ B) i).
+
+  Lemma instruction_cast_same tffi A B (i : syntax.instruction tffi A B) :
+    typer.instruction_cast A A B B i = Return _ i.
+  Proof.
+    unfold typer.instruction_cast.
+    rewrite stype_dec_same.
+    rewrite stype_dec_same.
+    reflexivity.
+  Qed.
+
+  Lemma instruction_cast_range_same tffi A B (i : syntax.instruction tffi A B) :
+    typer.instruction_cast_range A B B i = Return _ i.
+  Proof.
+    apply instruction_cast_same.
+  Qed.
+
+  Lemma instruction_cast_domain_same tffi A B (i : syntax.instruction tffi A B) :
+    typer.instruction_cast_domain A A B i = Return _ i.
+  Proof.
+    apply instruction_cast_same.
+  Qed.
+
+  Lemma untype_type_check_instruction tffi A B (i : syntax.instruction tffi A B) :
+    untype_type_spec _ _ _ i ->
+    typer.type_check_instruction typer.type_instruction (untype_instruction i) A B =
+    Return _ (existT _ tffi i).
+  Proof.
+    intro IH.
+    unfold typer.type_check_instruction.
+    rewrite IH.
+    simpl.
+    destruct tffi.
+    - rewrite tail_fail_change_range_same.
+      reflexivity.
+    - rewrite instruction_cast_range_same.
+      reflexivity.
+  Qed.
+
+  Lemma untype_type_check_instruction_no_tail_fail A B (i : syntax.instruction false A B) :
+    untype_type_spec _ _ _ i ->
+    typer.type_check_instruction_no_tail_fail typer.type_instruction (untype_instruction i) A B =
+    Return _ i.
+  Proof.
+    intro IH.
+    unfold typer.type_check_instruction_no_tail_fail.
+    rewrite IH.
+    simpl.
+    apply instruction_cast_range_same.
+  Qed.
+
+  Lemma untype_type_instruction_no_tail_fail A B (i : syntax.instruction false A B) :
+    untype_type_spec _ _ _ i ->
+    typer.type_instruction_no_tail_fail typer.type_instruction (untype_instruction i) A = Return _ (existT _ _ i).
+  Proof.
+    intro IH.
+    unfold typer.type_instruction_no_tail_fail.
+    rewrite IH.
+    reflexivity.
+  Qed.
+
+  Inductive IF_instruction : forall (A1 A2 A : Datatypes.list type), Set :=
+  | IF_i A : IF_instruction A A (bool ::: A)
+  | IF_NONE_i a A : IF_instruction A (a ::: A) (option a ::: A)
+  | IF_LEFT_i a b A : IF_instruction (a ::: A) (b ::: A) (or a b ::: A)
+  | IF_RIGHT_i a b A : IF_instruction (b ::: A) (a ::: A) (or a b ::: A)
+  | IF_CONS_i a A : IF_instruction (a ::: list a ::: A) A (list a ::: A).
+
+  Definition IF_instruction_to_instruction A1 A2 A (IFi : IF_instruction A1 A2 A) :
+    forall B tffa tffb,
+      syntax.instruction tffa A1 B ->
+      syntax.instruction tffb A2 B -> syntax.instruction (tffa && tffb) A B :=
+    match IFi with
+    | IF_i A => fun B ttffa tffb i1 i2 => syntax.IF_ i1 i2
+    | IF_NONE_i a A => fun B ttffa tffb i1 i2 => syntax.IF_NONE i1 i2
+    | IF_LEFT_i a b A => fun B ttffa tffb i1 i2 => syntax.IF_LEFT i1 i2
+    | IF_RIGHT_i a b A => fun B ttffa tffb i1 i2 => syntax.IF_RIGHT i1 i2
+    | IF_CONS_i a A => fun B ttffa tffb i1 i2 => syntax.IF_CONS i1 i2
+    end.
+
+  Lemma untype_type_branches tff1 tff2 A1 A2 A B
+        (i1 : syntax.instruction tff1 A1 B)
+        (i2 : syntax.instruction tff2 A2 B) IF_instr :
+    untype_type_spec _ _ _ i1 ->
+    untype_type_spec _ _ _ i2 ->
+    typer.type_branches typer.type_instruction
+                        (untype_instruction i1)
+                        (untype_instruction i2)
+                        A1 A2 A (IF_instruction_to_instruction A1 A2 A IF_instr) =
+    Return _ ((if (tff1 && tff2)%bool
+                 as b return syntax.instruction b A B -> typer.typer_result A
+               then
+                 fun i =>
+                   typer.Any_type _ (fun B' => tail_fail_change_range A B B' i)
+               else
+                 typer.Inferred_type _ B) (IF_instruction_to_instruction A1 A2 A IF_instr B tff1 tff2 i1 i2)).
+  Proof.
+    intros IH1 IH2.
+    unfold typer.type_branches.
+    rewrite IH1.
+    rewrite IH2.
+    simpl.
+    destruct tff1; destruct tff2; simpl.
+    - f_equal.
+      f_equal.
+      destruct IF_instr; simpl; unfold tail_fail_change_range; reflexivity.
+    - rewrite tail_fail_change_range_same.
+      reflexivity.
+    - rewrite tail_fail_change_range_same.
+      reflexivity.
+    - rewrite instruction_cast_range_same.
+      reflexivity.
+  Qed.
+
+  Ltac trans_refl t := transitivity t; [reflexivity|].
+
+  Fixpoint untype_type_data a (d : syntax.concrete_data a) :
+    typer.type_data (untype_data d) a = Return _ d
+  with
+  untype_type_instruction tffi A B (i : syntax.instruction tffi A B) :
+    untype_type_spec _ _ _ i.
+  Proof.
+    - destruct d; try reflexivity.
+      + admit.
+      + simpl.
+        unfold typer.type_data.
+        destruct (mtype_dec (C.get_contract_type cst) (Return _ a)).
+        * f_equal. f_equal.
+          apply Eqdep_dec.UIP_dec.
+          apply M_dec.
+          apply type_dec.
+        * congruence.
+      + simpl.
+        trans_refl (bind (fun x => bind (fun y => Return _ (@syntax.Pair a b x y)) (typer.type_data (untype_data d2) b)) (typer.type_data (untype_data d1) a)).
+        rewrite (untype_type_data _ d1).
+        rewrite (untype_type_data _ d2).
+        reflexivity.
+      + trans_refl (bind (fun x => Return _ (@syntax.Left a b x)) (typer.type_data (untype_data d) a)).
+        rewrite (untype_type_data _ d).
+        reflexivity.
+      + trans_refl (bind (fun x => Return _ (@syntax.Right a b x)) (typer.type_data (untype_data d) b)).
+        rewrite (untype_type_data _ d).
+        reflexivity.
+      + trans_refl (bind (fun x => Return _ (@syntax.Some_ a x)) (typer.type_data (untype_data d) a)).
+        rewrite (untype_type_data _ d).
+        reflexivity.
+      + pose (fix type_data_list (l : Datatypes.list concrete_data) :=
+                match l with
+                | nil => Return _ nil
+                | cons x l =>
+                  bind (fun x =>
+                          bind (fun l =>
+                                  Return (Datatypes.list (@syntax.concrete_data a)) (cons x l))
+                               (type_data_list l))
+                       (typer.type_data x a)
+                end) as type_data_list.
+        assert (forall l, type_data_list (List.map (fun x => untype_data x) l) = Return _ l).
+        * clear l.
+          intro l; induction l.
+          -- reflexivity.
+          -- simpl.
+             rewrite untype_type_data.
+             rewrite IHl.
+             reflexivity.
+        * trans_refl
+            (bind
+               (fun l => Return _ (@syntax.Concrete_list a l))
+               (type_data_list (List.map (fun x => untype_data x) l))).
+          rewrite H.
+          reflexivity.
+      + pose (fix type_data_set (l : Datatypes.list concrete_data) :=
+                match l with
+                | nil => Return _ nil
+                | cons x l =>
+                  bind (fun x =>
+                          bind (fun l =>
+                                  Return (Datatypes.list (@syntax.concrete_data a)) (cons x l))
+                               (type_data_set l))
+                       (typer.type_data x a)
+                end) as type_data_set.
+        assert (forall l, type_data_set (List.map (fun x => untype_data x) l) = Return _ l).
+        * clear l.
+          intro l; induction l.
+          -- reflexivity.
+          -- simpl.
+             rewrite untype_type_data.
+             rewrite IHl.
+             reflexivity.
+        * trans_refl
+            (bind
+               (fun l => Return _ (@syntax.Concrete_set a l))
+               (type_data_set (List.map (fun x => untype_data x) l))).
+          rewrite H.
+          reflexivity.
+      + pose (fix type_data_map (l : Datatypes.list concrete_data) :=
+                match l with
+                | nil =>
+                  Return
+                    (Datatypes.list
+                       (syntax.elt_pair
+                          (@syntax.concrete_data a)
+                          (@syntax.concrete_data b)))
+                    nil
+                | cons (Elt x y) l =>
+                  bind (fun x =>
+                          bind (fun y =>
+                                  bind (fun l =>
+                                          Return _ (cons (syntax.Elt _ _ x y) l))
+                                       (type_data_map l))
+                               (typer.type_data y b))
+                       (typer.type_data x a)
+                | _ => Failed _ Typing
+                end) as type_data_map.
+        assert (forall l, type_data_map (List.map (fun '(syntax.Elt _ _ x y) => Elt (untype_data x) (untype_data y)) l) = Return _ l).
+        * clear l.
+          intro l; induction l.
+          -- reflexivity.
+          -- simpl.
+             destruct a0.
+             rewrite untype_type_data.
+             rewrite untype_type_data.
+             rewrite IHl.
+             reflexivity.
+        * trans_refl (bind
+                          (fun l => Return _ (@syntax.Concrete_map a b l))
+                          (type_data_map (List.map (fun '(syntax.Elt _ _ x y) => Elt (untype_data x) (untype_data y)) l))).
+          rewrite H.
+          reflexivity.
+      + trans_refl
+          (bind
+             (fun '(existT _ tff i) => Return _ (syntax.Instruction _ (i : syntax.instruction _ _ _)))
+             (typer.type_check_instruction
+                typer.type_instruction
+                (untype_instruction i)
+                (cons a nil)
+                (cons b nil))).
+        rewrite untype_type_check_instruction; auto.
+      + admit.
+    - destruct i; try reflexivity; simpl.
+      + trans_refl
+          (bind (fun '(existT _ B i1) =>
+                   bind (fun r2 =>
+                           match r2 with
+                           | typer.Inferred_type _ C i2 =>
+                             Return _ (typer.Inferred_type _ _ (syntax.SEQ (i1 : syntax.instruction _ _ _) i2))
+                           | typer.Any_type _ i2 =>
+                             Return _ (typer.Any_type _ (fun C => syntax.SEQ i1 (i2 C)))
+                           end)
+                        (typer.type_instruction (untype_instruction i2) B))
+                (typer.type_instruction_no_tail_fail typer.type_instruction
+                                                     (untype_instruction i1) A)).
+        rewrite untype_type_instruction_no_tail_fail.
+        * simpl.
+          rewrite untype_type_instruction.
+          destruct tff; reflexivity.
+        * auto.
+      + trans_refl
+          (@typer.type_branches
+             typer.type_instruction
+             (untype_instruction i1)
+             (untype_instruction i2) _ _ _
+             (IF_instruction_to_instruction _ _ _ (IF_i A))).
+        rewrite untype_type_branches; auto.
+      + trans_refl
+          (bind (fun i => Return _ (@typer.Inferred_type _ _ (syntax.LOOP i)))
+           (typer.type_check_instruction_no_tail_fail
+              typer.type_instruction (untype_instruction i) A (bool ::: A))).
+        rewrite untype_type_check_instruction_no_tail_fail; auto.
+      + trans_refl
+          (bind (fun i => Return _ (@typer.Inferred_type _ _ (syntax.LOOP_LEFT i)))
+           (typer.type_check_instruction_no_tail_fail
+              typer.type_instruction (untype_instruction i) _ (or a b ::: A))).
+        rewrite untype_type_check_instruction_no_tail_fail; auto.
+      + trans_refl
+          (let A := a :: lambda a b :: C in
+           bind (fun i => Return _ (@typer.Inferred_type _ _ i))
+                (typer.instruction_cast_domain A A _ syntax.EXEC)).
+        simpl.
+        rewrite instruction_cast_domain_same.
+        reflexivity.
+      + admit.
+      + trans_refl
+          (bind (fun d => Return _ (@typer.Inferred_type A _ (syntax.PUSH a d)))
+                (typer.type_data (untype_data x) a)).
+        rewrite untype_type_data.
+        reflexivity.
+      + trans_refl
+          (bind (fun '(existT _ tff i) =>
+                   Return _ (@typer.Inferred_type _ (lambda a b ::: A) (syntax.LAMBDA a b i)))
+                (typer.type_check_instruction
+                   typer.type_instruction (untype_instruction i) (a :: nil) (b :: nil))).
+        rewrite untype_type_check_instruction; auto.
+      + destruct s as [v]; destruct v; reflexivity.
+      + destruct s as [v]; destruct v; reflexivity.
+      + destruct s as [v]; destruct v; reflexivity.
+      + destruct s as [a v]; destruct v; reflexivity.
+      + destruct s as [v]; destruct v; reflexivity.
+      + admit.
+      + admit.
+      + destruct s as [c v]; destruct v; reflexivity.
+      + destruct s as [c v]; destruct v; reflexivity.
+      + destruct s as [c v]; destruct v; reflexivity.
+      + destruct s as [c d v]; destruct v; reflexivity.
+      + admit.
+      + destruct i as [v]; destruct v; reflexivity.
+      + destruct i as [v]; destruct v; reflexivity.
+      + destruct i as [v]; destruct v; reflexivity.
+      + destruct i as [v]; destruct v.
+        * trans_refl
+            (let A := a ::: set a ::: S in
+             bind (fun i => Return _ (@typer.Inferred_type _ _ i))
+                  (typer.instruction_cast_domain
+                     A A _ (@syntax.MEM _ _ (mem_set a) _))).
+          simpl.
+          rewrite instruction_cast_domain_same.
+          reflexivity.
+        * trans_refl
+            (let A := key ::: map key val ::: S in
+             bind (fun i => Return _ (@typer.Inferred_type _ _ i))
+                  (typer.instruction_cast_domain
+                     A A _ (@syntax.MEM _ _ (mem_map key val) _))).
+          simpl.
+          rewrite instruction_cast_domain_same.
+          reflexivity.
+        * trans_refl
+            (let A := key ::: big_map key val ::: S in
+             bind (fun i => Return _ (@typer.Inferred_type _ _ i))
+                  (typer.instruction_cast_domain
+                     A A _ (@syntax.MEM _ _ (mem_bigmap key val) _))).
+          simpl.
+          rewrite instruction_cast_domain_same.
+          reflexivity.
+      + destruct i as [v]; destruct v.
+        * trans_refl
+          (let A := a ::: bool ::: set a :: S in
+           bind (fun i => Return _ (typer.Inferred_type _ _ i))
+                (typer.instruction_cast_domain
+                   A A _ (@syntax.UPDATE _ _ _ (update_set a) _))).
+          simpl.
+          rewrite instruction_cast_domain_same.
+          reflexivity.
+        * trans_refl
+            (let A := key ::: option val ::: map key val :: S in
+             bind (fun i => Return _ (typer.Inferred_type _ _ i))
+                  (typer.instruction_cast_domain
+                     A A _ (@syntax.UPDATE _ _ _ (update_map key val) _))).
+          simpl.
+          rewrite instruction_cast_domain_same.
+          reflexivity.
+        * trans_refl
+            (let A := key ::: option val ::: big_map key val :: S in
+             bind (fun i => Return _ (typer.Inferred_type _ _ i))
+                  (typer.instruction_cast_domain
+                     A A _ (@syntax.UPDATE _ _ _ (update_bigmap key val) _))).
+          simpl.
+          rewrite instruction_cast_domain_same.
+          reflexivity.
+      + destruct i as [c v]; destruct v.
+        * trans_refl
+            (bind (fun i => Return _ (@typer.Inferred_type _ _ (syntax.ITER i)))
+                  (typer.type_check_instruction_no_tail_fail typer.type_instruction (untype_instruction i0) (a ::: A) A)).
+          rewrite untype_type_check_instruction_no_tail_fail; auto.
+        * trans_refl
+            (bind (fun i => Return _ (@typer.Inferred_type _ _ (syntax.ITER i)))
+                  (typer.type_check_instruction_no_tail_fail typer.type_instruction (untype_instruction i0) (pair key val :: A) A)).
+          rewrite untype_type_check_instruction_no_tail_fail; auto.
+        * trans_refl
+            (bind (fun i => Return _ (@typer.Inferred_type _ _ (syntax.ITER i)))
+                  (typer.type_check_instruction_no_tail_fail typer.type_instruction (untype_instruction i0) (a :: A) A)).
+          rewrite untype_type_check_instruction_no_tail_fail; auto.
+      + destruct i as [c v]; destruct v.
+        * trans_refl
+            (let A := key ::: map key val :: S in
+             bind (fun i => Return _ (typer.Inferred_type _ _ i))
+                  (typer.instruction_cast_domain
+                     A A _ (@syntax.GET _ _ (get_map key val) _))).
+          simpl.
+          rewrite instruction_cast_domain_same.
+          reflexivity.
+        * trans_refl
+            (let A := key ::: big_map key val :: S in
+             bind (fun i => Return _ (typer.Inferred_type _ _ i))
+                  (typer.instruction_cast_domain
+                     A A _ (@syntax.GET _ _ (get_bigmap key val) _))).
+          simpl.
+          rewrite instruction_cast_domain_same.
+          reflexivity.
+      + destruct i as [a c v]; destruct v.
+        * trans_refl
+            (bind (fun r =>
+                     match r with
+                     | existT _ (b :: A') i =>
+                       bind (fun i => Return _ (@typer.Inferred_type _ _ (syntax.MAP i)))
+                            (typer.instruction_cast_range (pair key val :: A) (b :: A') (b :: A) i)
+                     | _ => Failed _ Typing
+                     end)
+                  (typer.type_instruction_no_tail_fail typer.type_instruction (untype_instruction i0) (pair key val ::: A))).
+          rewrite untype_type_instruction_no_tail_fail.
+          -- simpl.
+             rewrite instruction_cast_range_same.
+             reflexivity.
+          -- auto.
+        * trans_refl
+            (bind (fun r =>
+              match r with
+              | existT _ (b :: A') i =>
+                bind (fun i => Return _ (@typer.Inferred_type _ _ (syntax.MAP i)))
+                     (typer.instruction_cast_range (a :: A) (b :: A') (b :: A) i)
+              | _ => Failed _ Typing
+              end)
+                  (typer.type_instruction_no_tail_fail typer.type_instruction (untype_instruction i0) (a :: A))).
+          rewrite untype_type_instruction_no_tail_fail.
+          -- simpl.
+             rewrite instruction_cast_range_same.
+             reflexivity.
+          -- auto.
+      + trans_refl
+          (@typer.type_branches
+             typer.type_instruction
+             (untype_instruction i1)
+             (untype_instruction i2) _ _ _
+             (IF_instruction_to_instruction _ _ _ (IF_NONE_i a A))).
+        rewrite untype_type_branches; auto.
+      + trans_refl
+          (@typer.type_branches
+             typer.type_instruction
+             (untype_instruction i1)
+             (untype_instruction i2) _ _ _
+             (IF_instruction_to_instruction _ _ _ (IF_LEFT_i a b A))).
+        rewrite untype_type_branches; auto.
+      + trans_refl
+          (@typer.type_branches
+             typer.type_instruction
+             (untype_instruction i1)
+             (untype_instruction i2) _ _ _
+             (IF_instruction_to_instruction _ _ _ (IF_RIGHT_i a b A))).
+        rewrite untype_type_branches; auto.
+      + trans_refl
+          (let A := a :: list a :: S in
+           bind (fun i => Return _ (@typer.Inferred_type _ _ i))
+                (typer.instruction_cast_domain A A _ (syntax.CONS))).
+        simpl.
+        rewrite instruction_cast_domain_same.
+        reflexivity.
+      + trans_refl
+          (@typer.type_branches
+             typer.type_instruction
+             (untype_instruction i1)
+             (untype_instruction i2) _ _ _
+             (IF_instruction_to_instruction _ _ _ (IF_CONS_i a A))).
+        rewrite untype_type_branches; auto.
+      + trans_refl
+          (let A := option key_hash ::: mutez ::: g ::: S in
+           bind (fun '(existT _ tff i) =>
+                   bind (fun i => Return _ (@typer.Inferred_type _ _ i))
+                        (typer.instruction_cast_domain
+                           A A _
+                           (syntax.CREATE_CONTRACT g p i)))
+                (typer.type_check_instruction typer.type_instruction (untype_instruction i) (pair p g :: nil) (pair (list operation) g :: nil))).
+        simpl.
+        rewrite untype_type_check_instruction.
+        -- simpl.
+           rewrite instruction_cast_domain_same.
+           reflexivity.
+        -- auto.
+      + trans_refl
+          (let A := p ::: mutez ::: contract p ::: S in
+           bind (fun i => Return _ (@typer.Inferred_type _ _ i))
+                (typer.instruction_cast_domain A A _ syntax.TRANSFER_TOKENS)).
+        simpl.
+        rewrite instruction_cast_domain_same.
+        reflexivity.
+      + admit.
+      + admit.
+      + admit.
+      + admit.
+  Admitted.
+
+End untyper.
